cfrontend/BeePL_typesystem.v
@@ -307,13 +307,13 @@ Inductive well_formed_var (Gamma : ty_context) (Sigma : store_context) (bge : Be
                            Gamma ! x = Some t ->
                            (exists l' t' v, vm ! x = Some (l', t') /\
                            t = t' /\ PTree.get l' Sigma = Some t /\ 
-                                                  deref_addr bge t m l' Ptrofs.zero Full v)) ->
+                                                  deref_addr t m l' Ptrofs.zero Full v)) ->
                           well_formed_var Gamma Sigma bge vm m
 | store_well_typed_gvar : (forall x t,
                           Gamma ! x = Some t ->
                           (exists l' v, vm ! x = None /\ Genv.find_symbol bge x = Some l' /\ 
                                             PTree.get l' Sigma = Some t /\ 
-                                            deref_addr bge t m l' Ptrofs.zero Full v)) ->
+                                            deref_addr t m l' Ptrofs.zero Full v)) ->
                          well_formed_var Gamma Sigma bge vm m.
 
 (*** Well formed loc (coming from ref, not variables) ***)
